theories/ConvergentRefinement.v
@@ -1,0 +1,282 @@
+From Coq Require Export Morphisms RelationClasses Setoid Program.Equality.
+From ITree Require Export ITree ITreeFacts Eq.Rutt Props.Divergence Props.Finite.
+From Paco Require Import paco.
+From Coq Require Export Eqdep EqdepFacts.
+Require Import Lia.
+Require Export Refinement.
+
+Import Monads.
+Import MonadNotation.
+Local Open Scope monad_scope.
+
+Variant conv_refF {E : Type -> Type} {R : Type} (F : itree_spec E R -> Prop) : itree_spec' E R -> Prop :=
+  | conv_ref_RetF r : conv_refF F (RetF r)
+  | conv_ref_TauF t : F t -> conv_refF F (TauF t)
+  | conv_ref_existsF (A : Type) (k : A -> itree_spec E R) :
+    (forall a, F (k a) ) -> conv_refF F (VisF Spec_exists k)
+  | conv_ref_forallF (A : Type) (k : A -> itree_spec E R) :
+    A -> (forall a, F (k a)) -> conv_refF F (VisF Spec_forall k)
+.
+
+Definition conv_ref_ {E : Type -> Type} {R : Type} (F : itree_spec E R -> Prop) (t : itree_spec E R) :=
+  conv_refF F (observe t).
+
+Lemma monotone_conv_refF {E R} (ot : itree_spec' E R) sim sim' 
+      (LE : sim <1= sim')
+      (IN : conv_refF sim ot) :
+  conv_refF sim' ot.
+Proof. induction IN; constructor; auto. Qed.
+
+Lemma monotone_conv_ref_ {E R} : monotone1 (@conv_ref_ E R).
+Proof. red. intros. eapply monotone_conv_refF; eauto. Qed.
+
+Hint Resolve monotone_conv_ref_ : paco.
+
+Definition conv_ref {E R} : itree_spec E R -> Prop := paco1 conv_ref_ bot1.
+
+
+Lemma conv_ref_ret_bind E1 E2 R1 S R2 RE REAns RR r (t2 : itree_spec E2 R2) :
+  forall (t1 : itree_spec E2 S), 
+    conv_ref t1 ->
+    @refines E1 E2 R1 R2 RE REAns RR (Ret r) (t1 >> t2) ->
+    refines RE REAns RR (Ret r) t2.
+Proof.
+  intros t1 Ht1 Href. punfold Href. red in Href. cbn in Href.
+  punfold Ht1. red in Ht1. pstep. red. cbn.
+  remember (RetF r) as x. remember (t1 >> t2) as tbind.
+  assert (Htbind : tbind ≅ t1 >> t2). subst. reflexivity.
+  clear Heqtbind. punfold Htbind. red in Htbind.
+  hinduction Href before RR; intros; inv Heqx; use_simpobs.
+  - unfold observe in Htbind. cbn in Htbind. destruct (observe t1) eqn : Ht1';
+      inv Htbind; try inv CHECK.
+    setoid_rewrite <- H2. constructor. auto.
+  - assert (HDEC: (exists t1', observe t1 = TauF t1') \/ (exists r', observe t1 = RetF r') ).
+    { unfold observe in Htbind. cbn in Htbind. destruct (observe t1); eauto.
+      inv Htbind; inv CHECK. }
+    destruct HDEC as [[t1' Ht1']  | [r' Hr'] ].
+    + eapply IHHref with (t1 := t1'); eauto.
+      rewrite Ht1' in Ht1. inv Ht1. pclearbot. pstep_reverse.
+      assert (Tau phi ≅ t1 >> t2). pstep. auto.
+      symmetry in Ht1'. use_simpobs. rewrite Ht1' in H. rewrite bind_tau in H.
+      pinversion H; try inv CHECK. pclearbot. subst.
+      clear - REL. pclearbot. pstep_reverse.
+    + assert (Tau phi ≅ t1 >> t2). pstep. auto.
+      symmetry in Hr'. use_simpobs. rewrite Hr' in H.
+      rewrite bind_ret_l in H.
+      punfold H. red in H. cbn in H. inv H; try inv CHECK.
+      constructor. pclearbot. eapply IHHref; eauto.
+      pstep_reverse. rewrite Hr', bind_ret_l. clear - REL. pclearbot. auto.
+  - assert (HDEC : (exists k : A -> _, observe t1 = VisF Spec_forall k) \/ (exists r', observe t1 = RetF r') ).
+    {
+      unfold observe in Htbind. cbn in Htbind. destruct (observe t1); eauto.
+      inv Htbind; inv CHECK.
+      cbn in Htbind. inv Htbind. inj_existT. subst. eauto. }
+    destruct HDEC as [ [k Hk] | [r' Hr'] ].
+    + rewrite Hk in Ht1. inv Ht1. inj_existT. subst. pclearbot. rename X into a.
+      eapply H0 with (t1 := k a); eauto. pstep_reverse. Unshelve. all : auto.
+      assert (Vis Spec_forall kphi ≅ t1 >> t2). pstep. auto.
+      symmetry in Hk. use_simpobs. rewrite Hk in H1. rewrite bind_vis in H1.
+      pinversion H1. inj_existT. subst. clear - REL. pclearbot.
+      pstep_reverse.
+    + symmetry in Hr'. use_simpobs.
+      assert (Vis Spec_forall kphi ≅ t1 >> t2). pstep. auto.
+      rewrite Hr' in H1. rewrite bind_ret_l in H1.
+      pinversion H1; try inv CHECK. inj_existT. subst.
+      constructor. intros. clear - H REL. pclearbot.
+      rewrite itree_eta' at 1. pstep_reverse. rewrite <- REL. pstep. apply H.
+  -  assert (HDEC : (exists k : A -> _, observe t1 = VisF Spec_exists k) \/ (exists r', observe t1 = RetF r') ).
+    {
+      unfold observe in Htbind. cbn in Htbind. destruct (observe t1); eauto.
+      inv Htbind; inv CHECK.
+      cbn in Htbind. inv Htbind. inj_existT. subst. eauto. }
+    destruct HDEC as [ [k Hk] | [r' Hr'] ].
+    + rewrite Hk in Ht1. inv Ht1. inj_existT. subst. pclearbot.
+      eapply IHHref with (t1 := k a); eauto. pstep_reverse.
+      assert (Vis Spec_exists kphi ≅ t1 >> t2). pstep. auto.
+      symmetry in Hk. use_simpobs. rewrite Hk in H. rewrite bind_vis in H.
+      pinversion H. inj_existT. subst. clear - REL. pclearbot.
+      pstep_reverse.
+    + symmetry in Hr'. use_simpobs.
+      assert (Vis Spec_exists kphi ≅ t1 >> t2). pstep. auto.
+      rewrite Hr' in H. rewrite bind_ret_l in H.
+      pinversion H; try inv CHECK. inj_existT. subst. econstructor.
+      Unshelve. all : auto. clear - REL Href. pclearbot.
+      rewrite itree_eta' at 1. pstep_reverse. rewrite <- REL. pstep. apply Href.
+Qed.
+
+Global Instance conv_ref_eqit_proper E R b1 b2 : 
+  Proper (@eqit (SpecEvent E) R R eq b1 b2 ==> flip impl) conv_ref.
+Proof.
+  pcofix CIH.
+  intros t1 t2 Ht Ht2. pstep. red. punfold Ht2. red in Ht2.
+  punfold Ht. red in Ht.
+  hinduction Ht before R; intros; pclearbot; try (constructor; eauto).
+  - right. eapply CIH; eauto. inv Ht2. pclearbot. auto.
+  - inv Ht2. inj_existT. subst. constructor. right. pclearbot. eapply CIH; eauto.
+    apply REL. apply H0.
+    inj_existT. subst. constructor; auto. pclearbot. right. eapply CIH; eauto.
+    apply REL. apply H0.
+  - left. pstep. red. eapply IHHt; eauto.
+  - inv Ht2. pclearbot. punfold H0.
+Qed.
+
+Lemma padded_conv_ref_ret_bind E1 E2 R1 S R2 RE REAns RR r (t2 : itree_spec E2 R2) :
+  forall (t1 : itree_spec E2 S), 
+    conv_ref t1 ->
+    @padded_refines E1 E2 R1 R2 RE REAns RR (Ret r) (t1 >> t2) ->
+    padded_refines RE REAns RR (Ret r) t2.
+Proof.
+  intros t1 Ht1. unfold padded_refines. setoid_rewrite pad_ret.
+  setoid_rewrite pad_bind. intros. rewrite pad_eutt in Ht1. eapply conv_ref_ret_bind; eauto.
+Qed.
+
+Lemma conv_ref_bind E R S (k : R -> itree_spec E S) :
+  forall t, conv_ref t ->
+  (forall r, conv_ref (k r) ) ->
+   conv_ref (ITree.bind t k).
+Proof.
+  intros t Ht Hk. generalize dependent t. pcofix CIH. intros t Ht. punfold Ht. red in Ht.
+  pstep. red. unfold observe. cbn. inv Ht.
+  - pstep_reverse. eapply paco1_mon; try eapply Hk. intros. contradiction.
+  - constructor. right. pclearbot. eapply CIH; eauto.
+  - constructor. right. pclearbot. eapply CIH; apply H0.
+  - constructor; auto. right. pclearbot. eapply CIH; apply H0.
+Qed.
+
+Variant conv_ref_mrecF {E D : Type -> Type} {R : Type} (P : forall A, D A -> Prop) 
+        (F : itree_spec (D +' E) R -> Prop) : 
+  itree_spec' (D +' E) R -> Prop :=
+  | conv_ref_mrec_RetF r : conv_ref_mrecF P F (RetF r)
+  | conv_ref_mrec_TauF t : F t -> conv_ref_mrecF P F (TauF t)
+  | conv_ref_mrec_existsF (A : Type) (k : A -> itree_spec _ R) :
+    (forall a, F (k a) ) -> conv_ref_mrecF P F (VisF Spec_exists k)
+  | conv_ref_mrec_forallF (A : Type) (k : A -> itree_spec _ R) :
+    A -> (forall a, F (k a)) -> conv_ref_mrecF P F (VisF Spec_forall k)
+  | conv_ref_mrec_inlF (A : Type) (d : D A) (k : A -> itree_spec _ R) :
+    P A d ->
+    (forall a, F (k a) ) -> conv_ref_mrecF P F (VisF (Spec_vis (inl1 d) ) k)
+.
+
+Definition conv_ref_mrec_ {E D: Type -> Type} {R : Type} P (F : itree_spec (D +' E) R -> Prop) 
+           (t : itree_spec (D +' E) R) :=
+  conv_ref_mrecF P F (observe t).
+
+Lemma monotone_conv_ref_mrecF {E D R} P (ot : itree_spec' (D +' E) R) sim sim' 
+      (LE : sim <1= sim')
+      (IN : conv_ref_mrecF P sim ot) :
+  conv_ref_mrecF P sim' ot.
+Proof. induction IN; constructor; auto. Qed.
+
+Lemma monotone_conv_ref_mrec_ {E D R} P : monotone1 (@conv_ref_mrec_ E D R P ).
+Proof. red. intros. eapply monotone_conv_ref_mrecF; eauto. Qed.
+
+Hint Resolve monotone_conv_ref_mrec_ : paco.
+
+Definition conv_ref_mrec {E D R} P : itree_spec (D +' E) R -> Prop := paco1 (conv_ref_mrec_ P) bot1.
+
+Lemma conv_ref_mrec_bind E D R S P (k : R -> itree_spec (D +' E) S ) :
+  forall t, conv_ref_mrec P t ->
+  (forall r, conv_ref_mrec P (k r) ) ->
+   conv_ref_mrec P (ITree.bind t k).
+Proof.
+  intros t Ht Hk. generalize dependent t. pcofix CIH. intros t Ht.
+  pstep. red. unfold observe. cbn. punfold Ht. red in Ht.
+  inv Ht.
+  - pstep_reverse. eapply paco1_mon; try apply Hk. intros. contradiction.
+  - constructor. right. pclearbot. eapply CIH; eauto.
+  - constructor. right. pclearbot. eapply CIH; eauto. apply H0.
+  - constructor; auto. right. pclearbot. eapply CIH. apply H0.
+  - constructor. auto. pclearbot. right. eapply CIH. apply H1.
+Qed.
+
+(*may need a more general induction hype *)
+
+Section ConvRefMRec.
+Context (E D : Type -> Type).
+Context (Pre : forall A, D A -> Prop).
+Context (bodies : D ~> itree_spec (D +' E) ).
+Context (A : Type) (init : D A) (Hinit : Pre A init).
+Context (Hconv : forall A (d : D A), Pre A d -> conv_ref_mrec Pre (bodies A d)  ).
+
+Lemma conv_ref_interp_mrec_conv_ref:
+    forall t : itree_spec (D +' E) A, conv_ref_mrec Pre t -> conv_ref (interp_mrec_spec bodies t).
+Proof.
+  pcofix CIH. intros t Ht. punfold Ht. red in Ht.
+  pstep. red. unfold observe. cbn. inv Ht.
+  - constructor.
+  - constructor. right. eapply CIH; eauto. pclearbot. auto.
+  - constructor. pclearbot. right. eapply CIH; eauto. apply H0.
+  - constructor; auto. right. pclearbot. eapply CIH; eauto.
+    apply H0.
+  - constructor. right. eapply CIH. pclearbot. apply conv_ref_mrec_bind; auto.
+Qed.
+
+Lemma conv_ref_mrec_conv_ref : conv_ref (mrec_spec bodies init).
+Proof.
+  eapply conv_ref_interp_mrec_conv_ref. auto.
+Qed.
+
+
+
+End ConvRefMRec.
+
+Global Instance conv_ref_mrec_eqit_proper E D R b1 b2 P : 
+  Proper (@eqit (SpecEvent (D +' E)) R R eq b1 b2 ==> flip impl) (conv_ref_mrec P).
+Proof.
+  pcofix CIH.
+  intros t1 t2 Ht Ht2. pstep. red. punfold Ht2. red in Ht2.
+  punfold Ht. red in Ht.
+  hinduction Ht before R; intros; pclearbot; try (constructor; eauto).
+  - right. eapply CIH; eauto. inv Ht2. pclearbot. auto.
+  - inv Ht2; inj_existT; subst; pclearbot.
+    + constructor. right. eapply CIH; eauto. apply REL. apply H0.
+    + constructor; auto. right. eapply CIH. apply REL. apply H0.
+    + constructor; auto. right. eapply CIH. apply REL. apply H3.
+  - left. pstep. red. eapply IHHt; eauto.
+  - inv Ht2. pclearbot. punfold H0.
+Qed.
+
+Lemma conv_ref_mrec_forall E D R P A k :
+  A ->
+  (forall a : A, @conv_ref_mrec E D R P (k a) ) ->
+  conv_ref_mrec P (Vis Spec_forall k).
+Proof.
+  intros. pstep. constructor. auto. left. apply H.
+Qed.
+
+Lemma conv_ref_mrec_exists E D R P A k :
+  (forall a : A, @conv_ref_mrec E D R P (k a) ) ->
+  conv_ref_mrec P (Vis Spec_exists k).
+Proof.
+  intros. pstep. constructor. left. apply H.
+Qed.
+
+Lemma conv_ref_mrec_inl E D R P A k (d : D A) :
+  (P A d : Prop) ->
+  (forall a : A, @conv_ref_mrec E D R P (k a) ) ->
+  conv_ref_mrec P (Vis (Spec_vis (inl1 d)) k ).
+Proof.
+  intros. pstep. constructor. auto. left. apply H0.
+Qed.
+(*now I want a good reasoning principle for finding conv_ref*)
+
+    (*can infer *)
+  (* shouldn't need coinduction *)
+  
+
+
+(*
+
+Lemma monotone_satisfiesF {E R1 R2} (RR : R1 -> R2 -> Prop) ot1 (ot2 : itree_spec' E R2) sim sim' 
+  (LE : sim <2= sim' )
+  (IN : satisfiesF RR sim ot1 ot2) : 
+  satisfiesF RR sim' ot1 ot2.
+Proof.
+  induction IN; eauto.
+Qed.
+
+Lemma monotone_satisfies_ {E R1 R2} RR : monotone2 (@satisfies_ E R1 R2 RR).
+Proof. red. intros. eapply monotone_satisfiesF; eauto. Qed.
+
+Hint Resolve monotone_satisfies_ : paco.
+*)
