theories/MergePartial.v
@@ -1,0 +1,819 @@
+Require Import Coq.Lists.List Coq.Sorting.Permutation.
+
+From Coq Require Export Morphisms RelationClasses Setoid Program.Equality.
+From ITree Require Export ITree ITreeFacts Eq.Rutt Props.Divergence Props.Finite.
+From Paco Require Import paco.
+From Coq Require Export Eqdep EqdepFacts Logic.Classical.
+Require Import Lia.
+Require Export Refinement Merge ConvergentRefinement.
+
+Import Monads.
+Import MonadNotation.
+Local Open Scope monad_scope.
+
+Open Scope list_scope.
+
+
+Lemma or_spec_l E1 E2 RE REAns R1 R2 RR (t1 t2 : itree_spec E1 R1) (t3 : itree_spec E2 R2) : 
+  @padded_refines E1 E2 R1 R2 RE REAns RR t1 t3 ->
+  @padded_refines E1 E2 R1 R2 RE REAns RR t2 t3 ->
+  @padded_refines E1 E2 R1 R2 RE REAns RR (or_spec t1 t2) t3.
+Proof.
+  intros. unfold or_spec. unfold padded_refines in *.
+  rewrite pad_vis. pstep. constructor. intros [ | ]; constructor; pstep_reverse.
+Qed.
+
+Lemma or_spec_r E1 E2 RE REAns R1 R2 RR (t1 : itree_spec E1 R1) (t2 t3: itree_spec E2 R2) : 
+  (@padded_refines E1 E2 R1 R2 RE REAns RR t1 t2 \/
+  @padded_refines E1 E2 R1 R2 RE REAns RR t1 t3) ->
+  @padded_refines E1 E2 R1 R2 RE REAns RR t1 (or_spec t2 t3).
+Proof.
+  intros. unfold or_spec. unfold padded_refines in *.
+  rewrite pad_vis. pstep.
+  destruct H.
+  - econstructor. constructor. Unshelve. all : try (apply true). pstep_reverse.
+  - econstructor. constructor. Unshelve. all : try (apply false). pstep_reverse.
+Qed.
+
+Lemma spin_bind E R S k :  (@ITree.spin E R) >>= k ≅ @ITree.spin E S.
+Proof.
+  ginit. gcofix CIH. gstep. red. cbn. constructor.
+  gfinal. eauto.
+Qed.
+
+Lemma and_or_spec E R (t1 t2 : itree_spec E R) : 
+  padded_refines_eq eq (and_spec t1 t2) (or_spec t1 t2).
+Proof.
+  unfold and_spec, or_spec, padded_refines_eq, padded_refines.
+  setoid_rewrite pad_vis. pstep. red. cbn. econstructor. constructor.
+  Unshelve. all : try apply true. econstructor. cbn. constructor.
+  Unshelve. all : try apply true. pstep_reverse. 
+  enough (padded_refines_eq eq t1 t1). auto. reflexivity.
+Qed.
+
+Fixpoint trepeat {E R} (n : nat) (t : itree E R) : itree E unit :=
+  match n with
+  | 0 => Ret tt
+  | S m => t;; trepeat m t end.
+
+Lemma trepeat_Sn E R (n : nat) (t : itree E R) :
+  trepeat (S n) t ≅ t;; trepeat n t.
+Proof.
+  apply eqit_bind; reflexivity.
+Qed.
+
+Lemma trepeat_0 E R (t : itree E R) : 
+  trepeat 0 t ≅ Ret tt.
+Proof. reflexivity. Qed.
+
+Definition halve_spec_fix {E} : list nat -> itree_spec E (list nat * list nat) :=
+  rec_fix_spec (fun halve_spec_rec l =>
+                  n <- spec_exists nat;;
+                  trepeat n ( l' <- spec_exists (list nat);; halve_spec_rec l' );;
+                  halve_spec l
+               ).
+
+
+Theorem padded_refines_ret E1 E2 R1 R2 RE REAns RR r1 r2 :
+  (RR r1 r2 : Prop) ->
+  @padded_refines E1 E2 R1 R2 RE REAns RR (Ret r1) (Ret r2).
+Proof.
+  intros Hr. red. repeat rewrite pad_ret. pstep. constructor. auto.
+Qed.
+
+Theorem padded_refines_vis E1 E2 R1 R2 A B 
+        RE REAns RR (e1 : E1 A) (e2 : E2 B)
+        (k1 : A -> itree_spec E1 R1) (k2 : B -> itree_spec E2 R2) : 
+  (RE A B e1 e2 : Prop) -> 
+  (forall a b, (REAns A B e1 e2 a b : Prop) -> padded_refines RE REAns RR (k1 a) (k2 b) ) ->
+  padded_refines RE REAns RR (Vis (Spec_vis e1) k1) (Vis (Spec_vis e2) k2).
+Proof.
+  unfold padded_refines. setoid_rewrite pad_vis. intros.
+  pstep. constructor; auto. intros. left. pstep. constructor.
+  left. eapply H0; auto.
+Qed.
+
+Variant halve_call : forall A, callE (list nat) (list nat * list nat) A -> A -> Prop :=
+  | halve_call_i (l l1 l2: list nat) : 
+    Permutation l (l1 ++ l2) ->
+    (length l1 >= length l2 /\ (length l > length l1 \/ length l <= 1)) ->
+    halve_call _ (Call l) (l1,l2).
+
+Lemma halve_correct' E l : padded_refines_eq eq (@halve E l) (halve_spec_fix l).
+Proof.
+  eapply padded_refines_monot with (RE1 := eqE) 
+                                   (REAns1 := eqEAns) 
+                                   (RR1 := sub_eqEAns halve_call _ _ (Call l) (Call l) ); eauto.
+  { intros [l1 l2] [l3 l4]. intros. inv PR. inj_existT. subst. auto. }
+  eapply padded_refines_mrec with (REInv := eqE) 
+                                  (* in this post condition need to include *)
+                                  (REAnsInv := sub_eqEAns halve_call).
+  2 : constructor. intros.
+  eqE_inv H. clear l. destruct d2 as [l]. cbn.
+  destruct l as [ | a [ | b l] ].
+  - existssr 0. rewrite trepeat_0. rewrite bind_ret_l.
+    existssr (@nil nat). existssr (@nil nat). assertsr. reflexivity.
+    assertsr. cbn. lia.
+    apply padded_refines_ret. do 2 constructor. reflexivity.
+    cbn. lia. (*note reflexivity is not enough this is a subreflexive rel*)
+  - existssr 0. rewrite trepeat_0. rewrite bind_ret_l.
+    existssr (a :: nil). existssr (@nil nat). assertsr. reflexivity.
+    assertsr. cbn. lia. apply padded_refines_ret. do 2 constructor.
+    reflexivity. cbn. lia.
+  - cbn. existssr 1. rewrite trepeat_Sn. setoid_rewrite trepeat_0.
+    cbn. repeat rewrite bind_bind. existssr l.
+    eapply padded_refines_bind with (RR :=
+                                    sub_eqEAns halve_call (list nat * list nat) (list nat * list nat) (Call (l)) (Call (l))).
+    + unfold call_spec. apply padded_refines_vis. repeat constructor.
+      intros [l1 l2] r Hl12. inv Hl12. inj_existT. subst.
+      inv H5. inj_existT. subst. apply padded_refines_ret.
+      constructor. auto.
+    + intros [l1 l2] r2 Heq. inv Heq. inj_existT. subst.
+      inv H4. inj_existT. injection H5. intros. subst. 
+      rewrite bind_ret_l.
+      existssr (a :: l1). existssr (b :: l2). assertsr. 
+      { cbn. rewrite Permutation_app_comm. cbn.
+      rewrite H0. rewrite Permutation_app_comm. reflexivity. }
+      assertsr.
+      { cbn. rewrite H0. repeat rewrite app_length. lia. }
+      apply padded_refines_ret. do 2 constructor.
+      { cbn. rewrite Permutation_app_comm. cbn.
+      rewrite H0. rewrite Permutation_app_comm. reflexivity. }
+      cbn. repeat rewrite H0. repeat rewrite app_length. lia.
+Qed.
+(*
+Section ConvRef.
+Context (E D : Type -> Type).
+Context (Pre : forall A, D A -> Prop).
+Context (bodies : D ~> itree_spec (D +' E) ).
+Context (A : Type) (init : D A) (Hinit : Pre A init).
+Context (Hconv : forall A (d : D A), Pre A d -> )
+
+
+
+Context {A B: Type} {E : Type -> Type}.
+Context (body : ((A -> itree_spec (callE A B +' E) B) -> A -> itree_spec (callE A B +' E) B)).
+Context (Inv : A -> Prop).
+
+Lemma rec_fix_conv_rev : 
+  (* (forall a, Inv a -> conv_ref (body a) ) -> *)
+  forall a, Inv a -> conv_ref (rec_fix_spec body a).
+
+
+End ConvRef. *)
+
+Global Instance padded_refines_eq_itree E1 E2 R1 R2 RE REAns RR
+  : Proper (eq_itree eq ==> eq_itree eq ==> impl) 
+           (@padded_refines E1 E2 R1 R2 RE REAns RR).
+Proof.
+  repeat intro. assert (x ≈ y). rewrite H. reflexivity.
+  rewrite <- H2. assert (x0 ≈ y0). rewrite H0. reflexivity.
+  rewrite <- H3. auto.
+Qed.
+
+Lemma interp_mrec_spec_or  (E : Type -> Type) (R : Type) (D : Type -> Type) (ctx : forall T : Type, D T -> itree_spec (D +' E) T) 
+  (t1 t2 : itree_spec _ R)
+  : interp_mrec_spec ctx (or_spec t1 t2) ≅ or_spec (interp_mrec_spec ctx t1) (interp_mrec_spec ctx t2).
+Proof.
+  setoid_rewrite interp_mrec_spec'_exists. apply eqit_Vis. intros [ | ]; reflexivity.
+Qed.
+
+Lemma interp_mrec_spec_spin (E : Type -> Type) (R : Type) (D : Type -> Type) (ctx : forall T : Type, D T -> itree_spec (D +' E) T) :
+  interp_mrec_spec ctx ITree.spin ≅ @ITree.spin _ R.
+Proof.
+  pcofix CIH. pstep. red. cbn. constructor.
+  right. eauto.
+Qed.
+
+Lemma conv_ref_mrec_spin (E D : Type -> Type) (R : Type) (P : forall A : Type, D A -> Prop) : 
+  @conv_ref_mrec E D R P ITree.spin.
+Proof.
+  pcofix CIH. pstep. red. cbn. constructor.
+  eauto.
+Qed.
+
+Lemma conv_ref_mrec_ex (E D : Type -> Type) (R A : Type) (P : forall A : Type, D A -> Prop) k : 
+  (forall a, conv_ref_mrec P (k a)) ->
+  @conv_ref_mrec E D R P (Vis (@Spec_exists _ A) k ).
+Proof.
+  intros. pstep. constructor. left. apply H.
+Qed.
+
+(*should be able to generalize this to cany concrete tree *)
+Lemma or_spec_r_Ret_inv E1 E2 R1 R2 RE REAns RR r t2 t3 :
+  @padded_refines E1 E2 R1 R2 RE REAns RR (Ret r) (or_spec t2 t3) ->
+  padded_refines RE REAns RR (Ret r) t2 \/ padded_refines RE REAns RR (Ret r) t3.
+Proof.
+  intros Hor. unfold padded_refines in *. setoid_rewrite pad_ret in Hor.
+  setoid_rewrite pad_ret. setoid_rewrite pad_vis in Hor.
+  pinversion Hor. inj_existT. subst. inv H1. destruct a.
+  - left. pstep. auto.
+  - right. pstep. auto.
+Qed.
+
+Section SpecFix.
+  Context {A B: Type} {E : Type -> Type}.
+  Context (Pre : A -> Prop) (Post : A -> B -> Prop).
+  Context (prog : A -> itree_spec E B).
+
+  Context (Hprog : forall a, (exists b, prog a ≈ Ret b) \/ prog a ≈ ITree.spin).
+
+  Definition total_spec (a : A) : itree_spec E B :=
+    assume_spec (Pre a);;
+    b <- spec_exists B;;
+    assert_spec (Post a b);;
+    Ret b.
+
+  (* better for using as a final spec *)
+  Definition partial_spec (a : A) : itree_spec E B :=
+    or_spec (total_spec a) ITree.spin.
+  (* better for syntax driven solving *)
+  (**)
+
+  Definition partial_spec_fix : A -> itree_spec E B :=
+    rec_fix_spec (fun rec a => 
+                    assume_spec (Pre a);;
+                    (
+                      n <- spec_exists nat;;
+                      trepeat n (a' <- spec_exists A;; assert_spec (Pre a');; rec a' )
+                    );;
+                    b <- spec_exists B;;
+                    assert_spec (Post a b);;
+                    Ret b
+                 ).
+
+  Definition partial_spec_fix' : A -> itree_spec E B :=
+    rec_fix_spec (fun rec a => 
+                        assume_spec (Pre a);;
+                        (
+                          n <- spec_exists nat;;
+                          trepeat n (a' <- spec_exists A;; assert_spec (Pre a');; rec a' )
+                        );;
+                        or_spec (
+                            b <- spec_exists B;;
+                            assert_spec (Post a b);;
+                            Ret b)
+                        ITree.spin
+                 ).
+
+
+
+  Lemma partial_spec_fix_partial_spec_assume_succeed':
+    forall (a : A) (b : B),
+      Pre a ->
+      padded_refines_eq eq (Ret b) (partial_spec_fix' a) ->
+      padded_refines_eq eq (Ret b) (partial_spec a).
+  Proof.
+    intros a b Ha Hfix. unfold partial_spec_fix' in Hfix. cbn in Hfix.
+    repeat setoid_rewrite interp_mrec_spec_or in Hfix.
+
+    (*need an inversion principle for or spec *)
+    (*could use rewrite for interp_mrec_spec and or_spec *)
+    do 2 setoid_rewrite interp_mrec_spec_bind in Hfix. revert Hfix.
+    match goal with | |- context [ interp_mrec_spec ?f _ ] => set f as body end.
+    intro Hfix. 
+    assert (
+        padded_refines_eq eq (interp_mrec_spec body (or_spec (b <- spec_exists B;; _ <- assert_spec (Post a b);; Ret b) ITree.spin)) (partial_spec a)).
+    {
+      rewrite interp_mrec_spec_or. unfold partial_spec.
+      apply or_spec_l.
+      - apply or_spec_r. left. unfold total_spec.
+        assumesr. intros. repeat setoid_rewrite interp_mrec_spec_bind. 
+        normalize_interp_mrec_spec. setoid_rewrite interp_mrec_spec_ret.
+        setoid_rewrite bind_bind. setoid_rewrite bind_ret_l.
+        eapply padded_refines_bind. reflexivity.
+        intros. subst. eapply padded_refines_bind. reflexivity.
+        intros. subst. reflexivity.
+      - apply or_spec_r. right. rewrite interp_mrec_spec_spin. reflexivity.
+    } setoid_rewrite H in Hfix.
+    setoid_rewrite interp_mrec_spec_ret in Hfix.
+    match type of Hfix with padded_refines_eq eq _ ?t => set t as t1 end.
+    fold t1 in Hfix.
+    
+    assert (t1 ≈ (interp_mrec_spec body (trigger (@Spec_forall _ (Pre a) ) ) >>
+                 Ret tt >> 
+                  (interp_mrec_spec body
+           (ITree.bind (spec_exists nat)
+              (fun n : nat => trepeat n (ITree.bind (spec_exists A) (fun a' : A => 
+                       trigger (@Spec_exists _ (Pre a') ) >> Ret tt >> call_spec a'))))) >> partial_spec a)
+                 ).
+    {
+      unfold t1. repeat rewrite bind_bind.
+      apply eqit_bind. reflexivity. intro.
+      reflexivity.
+    }
+    rewrite H0 in Hfix. clear H0. 
+    (*might have dropped an important assumption *)
+    eapply padded_conv_ref_ret_bind; eauto.
+    normalize_interp_mrec_spec. cbn.
+    apply conv_ref_bind.
+    { pstep. red. cbn. constructor; auto. intros a0.
+          left. pstep. red. cbn. constructor. }
+    intros _.  setoid_rewrite bind_ret_l.
+    eapply conv_ref_interp_mrec_conv_ref.
+    Unshelve. 3 : { intros C c. destruct c. apply (Pre a0). }
+    - cbn.
+      intros. destruct d. cbn.
+      clear - H0 Ha. setoid_rewrite bind_bind. 
+      apply conv_ref_mrec_bind.
+      { pstep. red. cbn. constructor. auto. left.
+        pstep. constructor. }
+      intros _. rewrite bind_ret_l.
+      repeat rewrite bind_bind. unfold or_spec. setoid_rewrite bind_vis.
+      apply conv_ref_mrec_ex. intros n.
+      rewrite bind_ret_l.
+      eapply conv_ref_mrec_bind.
+      + induction n. cbn. pstep. constructor.
+        cbn. apply conv_ref_mrec_bind; intros; eauto.
+        apply conv_ref_mrec_bind. apply conv_ref_mrec_ex.
+        intros. pstep. constructor. intros.
+        rewrite bind_bind.
+        setoid_rewrite bind_vis.
+        apply conv_ref_mrec_ex. intros Hr.
+        repeat rewrite bind_ret_l. apply conv_ref_mrec_inl.
+        auto. intros. pstep. constructor.
+      + intros []. apply conv_ref_mrec_ex.
+        intros [ | ]; try apply conv_ref_mrec_spin.
+        setoid_rewrite bind_vis. apply conv_ref_mrec_ex.
+        intros. setoid_rewrite bind_ret_l. rewrite bind_bind. setoid_rewrite bind_vis.
+        apply conv_ref_mrec_ex. intros.
+        repeat rewrite bind_ret_l. pstep. constructor.
+    - setoid_rewrite bind_vis. setoid_rewrite bind_ret_l.
+      apply conv_ref_mrec_exists. intros n. clear - n Ha.
+      induction n. cbn. pstep. constructor.
+      cbn. eapply conv_ref_mrec_bind; eauto.
+      setoid_rewrite bind_bind. setoid_rewrite bind_ret_l. 
+      setoid_rewrite bind_vis.
+      apply conv_ref_mrec_exists. intros a0. rewrite bind_ret_l.
+      setoid_rewrite bind_vis. apply conv_ref_mrec_exists. intros Ha0.
+      rewrite bind_ret_l. apply conv_ref_mrec_inl. auto. intros. pstep. constructor.
+  Qed.
+
+  Lemma partial_spec_fix_partial_spec_assume_fail a :
+    ~ Pre a -> padded_refines_eq eq (prog a) (partial_spec a).
+  Proof.
+    intros HPre. apply or_spec_r.
+    left. assumesr. intros. contradiction.
+  Qed.
+
+  Lemma partial_spec_fix_partial_spec_assume_succeed:
+    forall (a : A) (b : B),
+      padded_refines_eq eq (Ret b) (partial_spec_fix a) ->
+      padded_refines_eq eq (Ret b) (partial_spec a).
+  Proof.
+    intros a b Hfix. 
+    apply or_spec_r. left. unfold total_spec.
+    assumesr. intros Ha.
+    unfold partial_spec_fix in Hfix.
+    do 2 setoid_rewrite interp_mrec_spec_bind in Hfix. revert Hfix.
+    match goal with | |- context [ interp_mrec_spec ?f _ ] => set f as body end.
+    intro Hfix. 
+    assert (interp_mrec_spec body (b <- spec_exists B;; _ <- assert_spec (Post a b);; Ret b) ≈ 
+                             (b <- spec_exists B;; _ <- assert_spec (Post a b);; Ret b)).
+    {
+      repeat setoid_rewrite interp_mrec_spec_bind.
+      normalize_interp_mrec_spec.
+      setoid_rewrite interp_mrec_spec_ret. cbn. reflexivity.
+    } setoid_rewrite H in Hfix.
+    (* need to manage diff between padded_refines and refines *)
+    cbn in Hfix. setoid_rewrite <- bind_bind in Hfix.
+    eapply padded_conv_ref_ret_bind; eauto.
+    setoid_rewrite interp_mrec_spec_ret. 
+    apply conv_ref_bind.
+    { pstep. red. cbn. constructor; auto. intros a0.
+          left. pstep. red. cbn. constructor. }
+    intros _. 
+    eapply conv_ref_interp_mrec_conv_ref.
+    Unshelve. 3 : { intros C c. destruct c. apply (Pre a0). }
+    - cbn.
+      intros. destruct d. cbn.
+      clear - H0 Ha. 
+      repeat rewrite bind_bind. setoid_rewrite bind_ret_l.
+      apply conv_ref_mrec_bind.
+      apply conv_ref_mrec_forall. auto. intros. pstep. constructor.
+      intros. rewrite <- bind_bind.
+      apply conv_ref_mrec_bind.
+      + rewrite bind_bind. apply conv_ref_mrec_bind. 
+        apply conv_ref_mrec_exists. intros. pstep. constructor.
+        intros n.
+        induction n; cbn. rewrite bind_ret_l. apply conv_ref_mrec_exists.
+        intros. pstep. constructor. rewrite bind_bind.
+        eapply conv_ref_mrec_bind; intros; eauto.
+        setoid_rewrite bind_vis. apply conv_ref_mrec_exists.
+        intros. setoid_rewrite bind_ret_l. rewrite bind_bind. setoid_rewrite bind_vis.
+        apply conv_ref_mrec_exists. intros. repeat rewrite bind_ret_l.
+        apply conv_ref_mrec_inl. auto. intros. pstep. constructor.
+      + intros b. rewrite bind_bind. setoid_rewrite bind_vis.
+        apply conv_ref_mrec_exists. intros HPost. repeat rewrite bind_ret_l.
+        pstep. constructor.
+    - setoid_rewrite bind_vis. setoid_rewrite bind_ret_l.
+      apply conv_ref_mrec_exists. intros n. clear - n Ha.
+      induction n. cbn. pstep. constructor.
+      cbn. eapply conv_ref_mrec_bind; eauto.
+      setoid_rewrite bind_bind. setoid_rewrite bind_ret_l. 
+      setoid_rewrite bind_vis.
+      apply conv_ref_mrec_exists. intros a0. rewrite bind_ret_l.
+      setoid_rewrite bind_vis. apply conv_ref_mrec_exists. intros Ha0.
+      rewrite bind_ret_l. apply conv_ref_mrec_inl. auto. intros. pstep. constructor.
+  Qed.
+
+
+  Lemma partial_spec_fix_partial_spec a :
+    (Pre a -> padded_refines_eq eq (prog a) (partial_spec_fix a)) ->
+    padded_refines_eq eq (prog a) (partial_spec a).
+  Proof.
+    intros Hfix.
+    destruct (Hprog a) as [ [b Hb] | Hspin].
+    - destruct (classic (Pre a) ) as [Ha | Ha]; auto.
+      + rewrite Hb. rewrite Hb in Hfix. 
+        apply partial_spec_fix_partial_spec_assume_succeed; auto.
+      + apply or_spec_r. left. assumesr. intros. contradiction.
+    - rewrite Hspin. apply or_spec_r. right. reflexivity.
+  Qed.
+
+  Lemma partial_spec_fix_partial_spec' a :
+    (Pre a -> padded_refines_eq eq (prog a) (partial_spec_fix' a)) ->
+    padded_refines_eq eq (prog a) (partial_spec a).
+  Proof.
+    intros Hfix.
+    destruct (Hprog a) as [ [b Hb] | Hspin].
+    - destruct (classic (Pre a) ) as [Ha | Ha]; auto.
+      + rewrite Hb. rewrite Hb in Hfix. 
+        apply partial_spec_fix_partial_spec_assume_succeed'; auto.
+      + apply or_spec_r. left. assumesr. intros. contradiction.
+    - rewrite Hspin. apply or_spec_r. right. reflexivity.
+  Qed.   
+
+  Variant pre_call : forall C, callE A B C -> Prop :=
+    | pre_call_intro (a : A) : Pre a -> pre_call B (Call a).
+  Variant post_call : forall C, callE A B C -> C -> Prop :=
+    | post_call_intro a b : Post a b -> post_call B (Call a) b.
+
+  (*
+  (* TODO : restructure this section so something like this can work *)
+  Lemma partial_spec_fix_partial_spec_inv a :
+    padded_refines (sub_eqE pre_call) (sub_eqEAns post_call) (sub_eq (Post a) ) 
+                   (prog a) (partial_spec_fix a).
+  *)
+  (* should work as long as Pre is inhabitted that allows *)
+  Lemma partial_spec_fix_spin a :
+    padded_refines_eq eq ITree.spin (partial_spec_fix a).
+  Proof.
+    unfold partial_spec_fix. setoid_rewrite interp_mrec_spec_bind.
+    setoid_rewrite interp_mrec_spec_assume. assumesr.
+    intros Ha. cbn. rewrite <-  bind_bind.
+    match goal with | |- padded_refines _ _ _ _ (interp_mrec_spec _ ( ITree.bind ?t1 ?t2) ) =>
+                        remember t2 as t end.
+    clear Heqt. generalize dependent t.
+    (* this seems like a good coind hyp*)
+    (* better solution might be to create a divergent refinement,
+       showing that there is a path that you can keep getting taus in 
+       then give that some kind of mrec rule
+     *)
+    pcofix CIH.
+  Admitted.
+
+  Lemma partial_spec_fix_spin' a :
+    padded_refines_eq eq ITree.spin (partial_spec_fix' a).
+  Proof.
+    unfold partial_spec_fix'. setoid_rewrite interp_mrec_spec_bind.
+    repeat normalize_interp_mrec_spec. assumesr. intros.
+    setoid_rewrite interp_mrec_spec_bind. 
+    setoid_rewrite interp_mrec_spec_bind.
+    normalize_interp_mrec_spec. 
+    match goal with |- context [ interp_mrec_spec ?body_ _  ] => set body_ as body end.
+    setoid_rewrite interp_mrec_spec_exists. existssr 0. cbn.
+    rewrite interp_mrec_spec_ret, bind_ret_l. rewrite interp_mrec_spec_or.
+    apply or_spec_r. right. rewrite interp_mrec_spec_spin. reflexivity.
+  Qed.
+
+
+End SpecFix.
+
+Opaque assume_spec.
+Opaque assert_spec.
+Opaque spec_forall.
+Opaque spec_exists.
+
+Lemma halve_spec_fix_correct' E l : 
+  padded_refines_eq eq (@halve E l) (partial_spec_fix (fun _ => True) 
+                                                   (fun l '(l1,l2) => Permutation l (l1 ++ l2) /\ 
+                               (length l1 >= length l2 /\ (length l > length l1 \/ length l <= 1)) ) l ).
+Proof.
+  eapply padded_refines_monot with (RE1 := eqE) 
+                                   (REAns1 := eqEAns) 
+                                   (RR1 := sub_eqEAns halve_call _ _ (Call l) (Call l) ); eauto.
+  { intros [l1 l2] [l3 l4]. intros. inv PR. inj_existT. subst. auto. }
+    eapply padded_refines_mrec with (REInv := eqE) 
+                                  (* in this post condition need to include *)
+                                  (REAnsInv := sub_eqEAns halve_call).
+  2 : constructor. intros.
+  eqE_inv H. clear l. destruct d2 as [l]. cbn.
+  destruct l as [ | a [ | b l] ].
+  - assumesr. intros _. rewrite bind_bind. existssr 0.
+    cbn. rewrite bind_ret_l. existssr (@nil nat,@nil nat).
+    assertsr. split. reflexivity. lia.
+    apply padded_refines_ret. do 2 constructor. reflexivity. cbn. lia.
+  - assumesr. intros _. rewrite bind_bind. existssr 0.
+    cbn. rewrite bind_ret_l. existssr (a :: nil, @nil nat).
+    assertsr. split. reflexivity. cbn. lia.
+    apply padded_refines_ret. do 2 constructor. reflexivity. cbn. lia.
+  - assumesr. intros _. rewrite bind_bind. existssr 1.
+    cbn. repeat rewrite bind_bind. existssr l.
+    repeat rewrite bind_bind.
+    assertsr. auto. setoid_rewrite bind_ret_l.
+    eapply padded_refines_bind with  (RR :=
+                                    sub_eqEAns halve_call (list nat * list nat) (list nat * list nat) (Call (l)) (Call (l))).
+    { apply padded_refines_vis. constructor. constructor. intros [l1 l2] b0 Hl12.
+      inv Hl12. inj_existT. subst. inv H5. inj_existT. subst.
+      apply padded_refines_ret. constructor. auto. }
+    intros [l1 l2] r Hl12. inv Hl12. inj_existT. subst. inv H4. inj_existT.
+    injection H5; intros; subst. existssr (a :: l1,b :: l2). assertsr.
+    split.
+    { cbn. rewrite Permutation_app_comm. cbn.
+      rewrite H0. rewrite Permutation_app_comm. reflexivity. }
+    { cbn. repeat rewrite H0. repeat rewrite app_length. lia. }
+    apply padded_refines_ret. constructor. constructor.
+    { cbn. rewrite Permutation_app_comm. cbn.
+      rewrite H0. rewrite Permutation_app_comm. reflexivity. }
+    { cbn. repeat rewrite H0. repeat rewrite app_length. lia. }
+ Qed.
+(* this requires lem *)
+Lemma halve_ret_spin E l : (exists l', @halve E l ≈ Ret l') \/ (@halve E l ≈ ITree.spin).
+Admitted.
+
+
+(* ok so there is a bunch of small things I still need to do but I think I have solved the problem *)
+Theorem halve_correct'' E l : padded_refines_eq eq (@halve E l) (partial_spec (fun _ => True) 
+                                                   (fun l '(l1,l2) => Permutation l (l1 ++ l2) /\ 
+                               (length l1 >= length l2 /\ (length l > length l1 \/ length l <= 1)) ) l).
+Proof.
+  eapply  partial_spec_fix_partial_spec. intros. apply halve_ret_spin.
+  intros _.
+  apply halve_spec_fix_correct'.
+Qed.
+
+Lemma sub_eqE_eq_type E P A B (ea : E A) (eb : E B) : sub_eqE P A B ea eb -> A = B.
+Proof.
+  intros. inv H. auto.
+Qed.
+
+Lemma sub_eqE_eq E P A (e1 : E A) (e2 : E A) : sub_eqE P A A e1 e2 -> e1 = e2 /\ P A e1.
+Proof.
+  intros. inv H. inj_existT. subst. auto.
+Qed.
+
+Lemma sub_eqEAns_eq_type E P A B (ea : E A) (eb : E B) a b : sub_eqEAns P A B ea eb a b -> A = B.
+Proof.
+  intros. inv H. auto.
+Qed.
+
+Lemma sub_eqEAns_eq E P A (e1 : E A) (e2 : E A) a1 a2 : sub_eqEAns P A A e1 e2 a1 a2 -> e1 = e2 /\ a1 = a2 
+                                                                                 /\ P A e1 a1.
+Proof.
+  intros. inv H. inj_existT. subst. auto.
+Qed.
+
+Ltac sub_eqE_inv H := eapply sub_eqE_eq_type in H as ?H; subst; eapply sub_eqE_eq in H as [?H ?H] ; subst.
+Ltac sub_eqEAns_inv H := apply sub_eqEAns_eq_type in H as ?H; subst; apply sub_eqEAns_eq in H as [?H [?H ?H] ]; subst.
+
+Section merge_correct.
+  Definition merge_pre '(l1,l2) := sorted l1 /\ sorted l2.
+  Definition merge_post '(l1,l2) l := sorted l /\ Permutation l (l1 ++ l2).
+
+  Theorem merge_correct'' E l1 l2 : padded_refines_eq eq (@Merge.merge E (l1,l2)) 
+                                                  (partial_spec merge_pre merge_post (l1,l2)).
+  Proof.
+    eapply partial_spec_fix_partial_spec. admit. (* proof that merge has no event *)
+    (* I should be able to assume here that Pre holds, because if it does not,
+       then I can easily *)
+    intros Hl12.
+    eapply padded_refines_monot with (RE1 := eqE ) 
+                                   (REAns1 := eqEAns) 
+                                   (RR1 := sub_eqEAns (post_call (merge_post) ) _ _ 
+                                                      (Call (l1,l2)) (Call (l1,l2)) ); eauto.
+    { intros. inv PR. inj_existT. subst. auto. }
+    eapply padded_refines_mrec with (REInv := sub_eqE (pre_call merge_pre) )
+                                    (REAnsInv := sub_eqEAns (post_call (merge_post) ) ).
+    2 : { do 2 constructor. auto. } 
+    intros. sub_eqE_inv H.
+    clear Hl12 l1 l2. destruct d2 as [ [ l1 l2] ]. inv H0. destruct H1 as [Hl1 Hl2].
+    cbn.
+    destruct l1; destruct l2.
+    - assumesr. intros _. repeat rewrite bind_bind. existssr (0). setoid_rewrite bind_ret_l.
+      existssr (@nil nat). assertsr. split; auto. apply padded_refines_ret.
+      repeat constructor.
+    - assumesr. intros _. repeat rewrite bind_bind. existssr 0. setoid_rewrite bind_ret_l.
+      existssr (n :: l2). assertsr. auto.  apply padded_refines_ret.
+      do 2 constructor. split; auto.
+    - assumesr. intros _. repeat rewrite bind_bind. existssr 0. setoid_rewrite bind_ret_l.
+      existssr (n :: l1). assertsr. split; auto. rewrite app_nil_r. auto. apply padded_refines_ret.
+      do 2 constructor. split. auto. rewrite app_nil_r. auto.
+    - rename n0 into m. destruct (Nat.leb n m) eqn : Hnm.
+      + cbn. assumesr. intros _. repeat rewrite bind_bind. existssr 1.
+        cbn. repeat rewrite bind_bind. existssr (l1, m :: l2). setoid_rewrite bind_bind. assertsr.
+        split; auto. eapply sorted_tail. eauto. apply padded_refines_bind with (RR := sub_eq (merge_post (l1, m :: l2) ) ).
+        { apply padded_refines_vis. do 3 constructor. split; auto. eapply sorted_tail. eauto.
+          intros. inv H. inj_existT. subst. sub_eqEAns_inv  H6.
+          inv H2. inj_existT. subst. apply padded_refines_ret. constructor. auto.
+        }
+        intros ? lm Hlm. inv Hlm. setoid_rewrite bind_ret_l. existssr (n :: lm).
+        assertsr.
+        { destruct H. split.
+          - admit. (*fact about sorted list *)
+          - rewrite H0. reflexivity. 
+        }
+        apply padded_refines_ret. destruct H. do 3 constructor.
+        * admit.
+        * setoid_rewrite H0. reflexivity.
+      + cbn. assumesr. intros _. repeat rewrite bind_bind. existssr 1.
+        cbn. repeat rewrite bind_bind. existssr (n :: l1, l2). setoid_rewrite bind_bind. assertsr.
+        split; auto. eapply sorted_tail. eauto. apply padded_refines_bind with (RR := sub_eq (merge_post (n :: l1,  l2) ) ).
+        { apply padded_refines_vis. do 3 constructor. split; auto. eapply sorted_tail. eauto.
+          intros. inv H. inj_existT. subst. sub_eqEAns_inv  H6.
+          inv H2. inj_existT. subst. apply padded_refines_ret. constructor. auto.
+        }
+        intros ? lm Hlm. inv Hlm. setoid_rewrite bind_ret_l. existssr (m :: lm).
+        assertsr.
+        { destruct H. split.
+          - admit. (*fact about sorted list *)
+          - rewrite H0. cbn. rewrite (Permutation_app_comm (l1) (m :: l2) ) .  cbn. rewrite Permutation_app_comm.
+            constructor.
+        }
+        apply padded_refines_ret. destruct H. do 3 constructor.
+        * admit.
+        * rewrite H0. cbn. rewrite (Permutation_app_comm (l1) (m :: l2) ) .  cbn. rewrite Permutation_app_comm.
+          constructor.
+ Admitted.
+
+End merge_correct.
+
+(* this should be contravariant, you can weaken the first and strengthen the second *)
+
+
+(*
+Instance test_le2 n : Proper (le ==> flip impl) (fun m => le m n).
+Proof.
+  repeat intro. subst. lia.
+Qed.
+                           
+Instance test_le1 : Proper (le ==> (flip le) ==> flip impl) le.
+Proof.
+  repeat intro. red in H0. lia.
+Qed.
+
+Instance test_le1' : Proper (le ==> (flip le) ==> impl) (flip le).
+Proof.
+  repeat intro. red in H0. red. red in H1. lia.
+Qed. *)
+(*
+Instance le_trans : Transitive le.
+Proof.
+  repeat intro. lia.
+Qed.
+
+Goal 1 <= 2 -> 2 <= 3 -> 1 <= 3.
+*)
+
+Global Instance padded_refines_sub_eq E R (RR : R -> R -> Prop) (P1 : forall A, E A -> Prop) (P2 : forall A, E A -> A -> Prop) :
+  Transitive RR ->
+  Transitive (padded_refines (sub_eqE P1) (sub_eqEAns P2) RR ).
+Proof.
+  intros HRR t1 t2 t3 Ht12 Ht23. unfold padded_refines in *.
+  eapply refines_monot; try eapply refinesTrans; eauto with solve_padded; try apply pad_is_padded.
+  - intros A B ea eb PR. inv PR. inj_existT. subst. sub_eqE_inv H3. auto.
+  - intros. sub_eqEAns_inv  PR. constructor. intros. destruct H. sub_eqE_inv H. 
+    exists x1. split; constructor; auto.
+  - intros. inv PR. etransitivity; eauto.
+Qed.
+
+Global Instance sub_eqEAns_trans E (P : forall A, E A -> A -> Prop) A (e : E A) : Transitive (sub_eqEAns P A A e e).
+Proof.
+  intros x y z Hxy Hyz. sub_eqEAns_inv Hxy. auto.
+Qed.
+
+(* I think I can save the rest for tomorrow*)
+
+(*
+Global Instance refines_proper_bind_RE E R RE REAns S :
+  Proper (@padded_refines E  R R eq ==> pointwise_relation _ (padded_refines_eq eq) ==> @padded_refines_eq E S S  eq ) ITree.bind.
+Proof.
+  repeat intro. subst. unfold padded_refines_eq in *. eapply padded_refines_bind; eauto.
+  intros; subst. auto.
+Qed.
+*)
+
+(*do I need the proper instances? Probably *)
+
+Global Instance  padded_refines_eq_gen E1 E2 R1 R2 RE REAns RR : Proper (padded_refines_eq eq ==> flip (padded_refines_eq eq) ==> flip impl )
+                                                                (@padded_refines E1 E2 R1 R2 RE REAns RR).
+Proof.
+  intros t1 t2 Ht12 t3 t4 Ht43. red in Ht43. intro.
+  unfold padded_refines_eq, padded_refines in *. rename H into H24.
+  specialize @refinesTrans with (E1 := E1) (E2 := E1) (E3 := E2) (RE1 := eqE) (RE2 := RE) as Htrans.
+  eapply Htrans in Ht12; eauto; try apply pad_is_padded. clear Htrans.
+  specialize @refinesTrans with (E1 := E1) (E2 := E2) (E3 := E2) (RE1 := rcomposeE eqE RE) (RE2 := eqE) as Htrans.
+  eapply Htrans in Ht12; eauto; try apply pad_is_padded. eapply refines_monot; try eapply Ht12.
+  { intros. destruct PR. destruct H. eqE_inv H. eqE_inv H0. auto. }
+  { intros. econstructor. intros. destruct H. eqE_inv H0. 
+    inv H. inj_existT. subst. eqE_inv H4. exists x1. split. 2 : constructor.
+    constructor. intros. destruct H. eqE_inv H. exists x0. split; auto. constructor.
+  }
+  { intros. inv PR. inv REL1. auto. }
+Qed.
+  (* this is maybe a tad more subtle then I realized, does it require transitivity?,
+     that would not be problematic for these relations because there seem to be PER's
+
+   *)
+
+Lemma or_spec_bind_l  E1 E2 R1 S R2 RE REAns RR (t1 t2 : itree_spec E1 S) (k : S -> itree_spec E1 R1) (t3 : itree_spec E2 R2) : 
+  padded_refines RE REAns RR (ITree.bind t1 k) t3 ->
+  padded_refines RE REAns RR (ITree.bind t2 k) t3 ->
+  padded_refines RE REAns RR (ITree.bind (or_spec t1 t2) k) t3.
+Proof.
+  unfold padded_refines. intros. setoid_rewrite bind_vis. setoid_rewrite pad_vis.
+  pstep. constructor. intros [ | ]; constructor; pstep_reverse.
+Qed.
+
+Section sort_correct.
+  Definition sort_pre (l : list nat) := True.
+  Definition sort_post (l l' : list nat) := Permutation l l' /\ sorted l'.
+
+  Theorem sort_correct' E l : padded_refines_eq eq (@sort E l) (partial_spec sort_pre sort_post l).
+  Proof.
+    eapply partial_spec_fix_partial_spec'. admit.
+    intros _.
+    eapply padded_refines_monot with (RE1 := eqE ) 
+                                   (REAns1 := eqEAns) 
+                                   (RR1 := sub_eqEAns (post_call (sort_post) ) _ _ 
+                                                      (Call (l)) (Call (l)) ); eauto.
+    { intros. sub_eqEAns_inv  PR. auto. }
+    eapply padded_refines_mrec with (REInv := sub_eqE (pre_call sort_pre) )
+                                    (REAnsInv := sub_eqEAns (post_call (sort_post) ) ).
+    2 : { repeat constructor. }
+    intros. clear l. sub_eqE_inv  H. destruct d2. inv H0.
+    cbn. destruct (Nat.leb (length l) 1 ) eqn : Hlen.
+    - assumesr. intros _. repeat rewrite bind_bind. existssr 0.
+      cbn. rewrite bind_ret_l. apply or_spec_r. left.
+      existssr l. 
+      assert (sort_post l l).
+      { destruct l. split; auto. constructor. destruct l. split; auto.
+        constructor. discriminate. }
+      assertsr. auto. apply padded_refines_ret. do 2 constructor. auto.
+    - rewrite halve_correct''. 
+      (* here I really want to push the or_spec left, probably only works if only quantifiers,
+         if I can get past this then it should work *)
+
+      unfold partial_spec, total_spec. rewrite or_spec_bind.
+      apply or_spec_l.
+      2 : { setoid_rewrite spin_bind. 
+            assumesr. intros _ . repeat rewrite bind_bind. existssr 0.
+            cbn. rewrite bind_ret_l. apply or_spec_r. right.
+            apply padded_refines_spin.
+          }
+      setoid_rewrite bind_bind at 1. assumesl. auto.  setoid_rewrite bind_bind at 1.
+      existssl. intros [l1 l2]. setoid_rewrite bind_bind at 1. assertsl.
+      intros Hl12. rewrite bind_ret_l.
+      (* now I really need to push the or_spec further because in order to get to the 
+         merge call (which itself might diverge , unless I actually  I need to just add more off ramps with o) *)
+
+      setoid_rewrite bind_bind. assumesr. intros _ .
+      existssr 2. cbn. repeat rewrite bind_bind.
+      existssr l1. rewrite bind_bind. assertsr.
+      auto. apply padded_refines_bind with (RR := sub_eq (sort_post l1) ).
+      { apply padded_refines_vis. repeat constructor.
+        intros. inv H. inj_existT. subst. sub_eqEAns_inv H7.
+        subst. apply padded_refines_ret. constructor. inv H3. inj_existT.
+        subst. auto.
+      }
+      intros ? l1s Hl1s. inv Hl1s.
+      repeat rewrite bind_bind.
+      existssr l2. repeat rewrite bind_bind. assertsr.
+      auto. apply padded_refines_bind with (RR := sub_eq (sort_post l2) ).
+      {
+        apply padded_refines_vis. repeat constructor. intros.
+        inv H0. inj_existT. subst. sub_eqEAns_inv H8.
+        subst. apply padded_refines_ret. constructor. inv H3. inj_existT.
+        subst. auto. }
+      intros ? l2s Hl2s. inv Hl2s. rewrite bind_ret_l.
+      rewrite merge_correct''. unfold partial_spec.
+      apply or_spec_l.
+      2 : { apply or_spec_r. right. apply padded_refines_spin. } (*same lemma as before*)
+      apply or_spec_r. left. unfold total_spec. cbn. red in H. red in H0.
+      assumesl. tauto.
+      existssl. intros ls. assertsl. intros Hls. destruct H. destruct H0. 
+      destruct Hls. existssr ls. assertsr.
+      split; auto.
+      destruct Hl12. rewrite H6, H, H0, H5. reflexivity.
+      apply padded_refines_ret.
+      constructor. split; auto.
+      destruct Hl12. 
+      split; auto.
+      rewrite H6, H, H0, H5. reflexivity.
+Admitted.
+
+End sort_correct.
+
+(*
+Theorem merge
+*)
